Notations.v
@@ -336,26 +336,42 @@ Notation "x `[ msb : lsb ]" := (ConstExtract ltac:(let y := eval simpl in (Z.sub
                                                             in exact y) lsb x)
                                  (msb at level 0, only parsing): guru_scope.
 
+Class __EvalRegPath (t : Tree DomainElem) (path : string) := __evalRegPath : RegPath t.
+#[global] Hint Extern 1 (__EvalRegPath ?t ?path) =>
+  let p := eval cbn in (getRegPathTree t path) in exact p : typeclass_instances.
+
+Class __EvalSendPath (t : Tree DomainElem) (path : string) := __evalSendPath : SendPath t.
+#[global] Hint Extern 1 (__EvalSendPath ?t ?path) =>
+  let p := eval cbn in (getSendPathTree t path) in exact p : typeclass_instances.
+
+Class __EvalMemPath (t : Tree DomainElem) (path : string) := __evalMemPath : MemPath t.
+#[global] Hint Extern 1 (__EvalMemPath ?t ?path) =>
+  let p := eval cbn in (getMemPathTree t path) in exact p : typeclass_instances.
+
+Class __EvalRecvPath (t : Tree DomainElem) (path : string) := __evalRecvPath : RecvPath t.
+#[global] Hint Extern 1 (__EvalRecvPath ?t ?path) =>
+  let p := eval cbn in (getRecvPathTree t path) in exact p : typeclass_instances.
+
 Notation "'RegRead' letv <- name 'in' t ; cont" :=
-  (ReadReg (Stringify letv) (getRegPathTree t name) (fun letv => cont)) (at level 20, letv name): guru_scope.
+  (ReadReg (Stringify letv) (match tt return __EvalRegPath t name with _ => _ end) (fun letv => cont)) (at level 20, letv name): guru_scope.
 
 Notation "'RegWrite' name 'in' t <- v ; cont" :=
-  (WriteReg (getRegPathTree t name) v cont) (at level 20): guru_scope.
+  (WriteReg (match tt return __EvalRegPath t name with _ => _ end) v cont) (at level 20): guru_scope.
 
 Notation "'MemReadRq' name 'in' t ! p <- i ; cont" :=
-  (ReadRqMem (getMemPathTree t name) i (@Build_FinType (getMemFromPath (getMemPathTree t name)).(memPort) p I) cont) (at level 20): guru_scope.
+  (ReadRqMem (match tt return __EvalMemPath t name with _ => _ end) i (@Build_FinType (getMemFromPath (match tt return __EvalMemPath t name with _ => _ end)).(memPort) p I) cont) (at level 20): guru_scope.
 
 Notation "'MemReadRp' letv <- name 'in' t ! p ; cont" :=
-  (ReadRpMem (Stringify letv) (getMemPathTree t name) (@Build_FinType (getMemFromPath (getMemPathTree t name)).(memPort) p I) (fun letv => cont)) (at level 20, letv name): guru_scope.
+  (ReadRpMem (Stringify letv) (match tt return __EvalMemPath t name with _ => _ end) (@Build_FinType (getMemFromPath (match tt return __EvalMemPath t name with _ => _ end)).(memPort) p I) (fun letv => cont)) (at level 20, letv name): guru_scope.
 
 Notation "'MemWrite' name 'in' t ! i <- v ; cont" :=
-  (WriteMem (getMemPathTree t name) i v cont) (at level 20): guru_scope.
+  (WriteMem (match tt return __EvalMemPath t name with _ => _ end) i v cont) (at level 20): guru_scope.
 
 Notation "'Put' name 'in' t <- v ; cont" :=
-  (Send (getSendPathTree t name) v cont) (at level 20): guru_scope.
+  (Send (match tt return __EvalSendPath t name with _ => _ end) v cont) (at level 20): guru_scope.
 
 Notation "'Get' letv <- name 'in' t ; cont" :=
-  (Recv (Stringify letv) (getRecvPathTree t name) (fun letv => cont)) (at level 20, letv name): guru_scope.
+  (Recv (Stringify letv) (match tt return __EvalRecvPath t name with _ => _ end) (fun letv => cont)) (at level 20, letv name): guru_scope.
 
 Notation "'Let' letv : k' <- e ; cont" :=
   (LetExp (Stringify letv) (k' := k') e (fun letv => cont)) (at level 20, letv name): guru_scope.
